Removed some proof

Increment-only_counter/App.fst
@@ -92,7 +92,7 @@ let concrete_merge_pre lca a b : prop
 
 // concrete merge operation
 let concrete_merge (lca:concrete_st) (s1:concrete_st) (s2:concrete_st{concrete_merge_pre lca s1 s2}) 
-  : concrete_st = s1 + s2 - lca
+  : (r:concrete_st{(lca = s1 ==> r = s2) /\ (lca = s2 ==> r = s1)}) = s1 + s2 - lca
 
 #push-options "--z3rlimit 100"
 let merge_inv_prop (lca s1 s2:st)
@@ -110,8 +110,11 @@ let merge_inv_prop (lca s1 s2:st)
                       concrete_merge_pre (v_of lca) (v_of (inverse_st s1)) (v_of s2)) /\
                     (last (resolve_conflict last1 last2) <> last1 ==>
                       concrete_merge_pre (v_of lca) (v_of s1) (v_of (inverse_st s2))))) =
+  let _, last1 = un_snoc (ops_of s1) in
+  let _, last2 = un_snoc (ops_of s2) in
+  lastop_neq (ops_of lca) (ops_of s1) (ops_of s2);
+  resolve_conflict_prop last1 last2;
   lem_foldl init_st (ops_of lca); 
-  lem_foldl init_st (ops_of s1);
   lem_foldl init_st (ops_of (inverse_st s2))
                       
 let linearizable_s1_0 (lca s1 s2:st)
@@ -124,8 +127,7 @@ let linearizable_s1_0 (lca s1 s2:st)
                 (forall id id1. mem_id id (ops_of lca) /\ mem_id id1 (diff (ops_of s2) (ops_of lca)) ==> lt id id1) /\
                 (forall id. mem_id id (diff (ops_of s1) (ops_of lca)) ==> not (mem_id id (diff (ops_of s2) (ops_of lca)))) /\
                 foldl_prop (v_of lca) (diff (ops_of s2) (ops_of lca)))
-      (ensures v_of s2 == concrete_merge (v_of lca) (v_of s1) (v_of s2)) =
-  lem_foldl init_st (ops_of s2)
+      (ensures v_of s2 == concrete_merge (v_of lca) (v_of s1) (v_of s2)) = ()
 
 let linearizable_s2_0 (lca s1 s2:st)
   : Lemma 
@@ -138,8 +140,7 @@ let linearizable_s2_0 (lca s1 s2:st)
                 (forall id id1. mem_id id (ops_of lca) /\ mem_id id1 (diff (ops_of s2) (ops_of lca)) ==> lt id id1) /\
                 (forall id. mem_id id (diff (ops_of s1) (ops_of lca)) ==> not (mem_id id (diff (ops_of s2) (ops_of lca)))) /\
                 foldl_prop (v_of lca) (diff (ops_of s1) (ops_of lca)))
-      (ensures v_of s1 == concrete_merge (v_of lca) (v_of s1) (v_of s2)) =
-  lem_foldl init_st (ops_of s1)
+      (ensures v_of s1 == concrete_merge (v_of lca) (v_of s1) (v_of s2)) = ()
 
 let lem_add (lca s1 s2:nat)
   : Lemma (ensures s1 + (s2 - 1) - lca + 1 = s1 + s2 - lca)
